The **Fibonacci numbers**, commonly denoted `F(n)` form a sequence, called the **Fibonacci sequence**, such that each number is the sum of the two preceding ones, starting from `0` and `1`. That is,

```
F(0) = 0,   F(1) = 1
F(N) = F(N - 1) + F(N - 2), for N > 1.
```

Given `N`, calculate `F(N)`.



动态规划加备忘录

```java
class Solution {
    public int fib(int n) {
        if(n<1) return 0;
        int pre=1;
        int cur=1;
        if(n==1 || n==2)
            cur=1;
        for(int i=3;i<=n;++i){
            int sum=cur+pre;
            pre=cur;
            cur=sum;
        }
        return cur;
    }
}
```



动态规划

```java
class Solution {
    public int fib(int n) {
        if(n<1) return 0;
        if(n==1 || n==2) return 1;
        int[] dp=new int[n+1];
        dp[1]=dp[2]=1;
        for(int i=3;i<n+1;++i){
            dp[i]=dp[i-2]+dp[i-1];
        }
        return dp[n];
    }
}
```



自顶向下的递归

```java
class Solution {
    public int fib(int N) {
        if(N<1) return 0;
        int[] ans=new int[N+1];
        return helper(N,ans); 
        
    }
    public int helper(int N, int[] ans){
        if(N==1 || N==2)
            return 1;
        if(ans[N]!=0)
            return ans[N];
        ans[N]=helper(N-1,ans)+helper(N-2,ans);
        return ans[N];
    }
}
```

